wip

src/graph/dijkstra.v
@@ -1,17 +1,51 @@
-From mathcomp Require Import ssreflect ssrbool ssrnat fintype fingraph seq.
+From mathcomp Require Import ssreflect ssrbool ssrnat eqtype fintype fingraph seq.
 Require Recdef.
-Require Import neko.heap.leftiest.
+Require neko.heap.leftist.
+Require Import neko.ordering.
 
-Section Dijkstra.
+Module Dijkstra.
   Parameter V: finType.
-  Parameter e: rel V.
-  Definition cost := nat.
-  Parameter c: V -> V -> cost.
+  Parameter g: V -> seq V.
+  Definition Cost: Type := nat.
+  Parameter cost: V -> V -> Cost.
 
-  Definition cnode: Type := V * cost.
+  Definition cnode: Type := V * Cost.
   Definition cpath: Type := seq cnode.
 
-  Function dijkstra (s: V): cpath :=
-    
+  Module Pair <: leftist.S.
+    Definition T: Type := nat * cpath.
+    Definition leT (x y: T) :=
+      let '(x', _) := x in
+      let '(y', _) := y in
+      x' <= y'.
+
+    Instance leT_total_preorder: TotalPreOrder leT.
+    Proof.
+      constructor.
+      constructor.
+      - case => ? _ /=; exact: leqnn.
+      - case => ? ?; case => ? ?; case => ? ? /=; exact: leq_trans.
+      - case => ? ?; case => ? ? /=; exact: leq_total.
+    Defined.
+  End Pair.
+
+  Module Import pqueue := leftist.LeftistHeap Pair.
+
+  Definition lt_pair' (vs_q1 vs_q2: seq V * tree) :=
+    let '(vs1, q1) := vs_q1 in
+    let '(vs2, q2) := vs_q2 in
+    (seq.size vs1 < seq.size vs2) || ((seq.size vs1 == seq.size vs2) && (size q1 < size q2)) = true.
+
+  Function dijkstra' (vs_q: seq V * tree) {wf lt_pair' vs_q}: cpath :=
+    let '(vs, q) := vs_q in
+    match split_min q with
+    | Split_empty => [:: ]
+    | Split_min_rest m q' =>
+      if m is (_, [:: (v, d) & _ ])
+      then
+        dijkstra' (vs, q')
+      else
+        [:: ]
+    end.
 
 End Dijkstra.
