src/heap/leftist.v
@@ -3,8 +3,12 @@ Require Recdef.
 
 Require Import neko.ordering.
 
-Module LeftistHeap (Import M: TOTAL_ORDER).
+Module Type S.
+  Parameters (T: Type) (leT: rel T).
+  Axiom leT_total_preorder: TotalPreOrder leT.
+End S.
 
+Module LeftistHeap(Import O: S).
   Create HintDb leftist.
   Ltac leftist_simpl :=
     simpl;
@@ -45,39 +49,41 @@ Module LeftistHeap (Import M: TOTAL_ORDER).
     | (Node l1 x1 r1 _ as t1, Node l2 x2 r2 _ as t2) =>
       if leT x1 x2
       then
-        let t := pair_merge (r1, t2) in
-        let kl := rank l1 in
-        let kr := rank t in
-        if kl <= kr then Node t x1 l1 kl.+1 else Node l1 x1 t kr.+1
+        let t1' := pair_merge (r1, t2) in
+        let t2' := l1 in
+        let k1' := rank t1' in
+        let k2' := rank t2' in
+        if k1' <= k2' then Node t1' x1 t2' k1'.+1 else Node t2' x1 t1' k2'.+1
       else
-        let t := pair_merge (t1, l2) in
-        let kl := rank t in
-        let kr := rank r2 in
-        if kl <= kr then Node t x2 r2 kl.+1 else Node r2 x2 t kr.+1
+        let t1' := pair_merge (t1, r2) in
+        let t2' := l2 in
+        let k1' := rank t1' in
+        let k2' := rank t2' in
+        if k1' <= k2' then Node t1' x2 t2' k1'.+1 else Node t2' x2 t1' k2'.+1
     end.
   Proof.
-    all: move => * /=; apply/ltP.
-      by rewrite ltn_add2r ltnS leq_addl.
-      by rewrite ltn_add2l ltnS leq_addr.
+    all: by move => * /=; apply/ltP; rewrite (ltn_add2r, ltn_add2l) ltnS leq_addl.
   Qed.
 
   Definition merge t1 t2 := pair_merge (t1, t2).
 
   Lemma merge_equation t1 t2:
-    merge t1 t2 = match t1, t2 with
-                  | Leaf, t | t, Leaf => t
-                  | Node l1 x1 r1 _, Node l2 x2 r2 _ =>
-                    if leT x1 x2
-                    then
-                      let t := merge r1 t2 in
-                      let kl := rank l1 in
-                      let kr := rank t in
-                      if kl <= kr then Node t x1 l1 kl.+1 else Node l1 x1 t kr.+1
-                    else
-                      let t := merge t1 l2 in
-                      let kl := rank t in
-                      let kr := rank r2 in
-                      if kl <= kr then Node t x2 r2 kl.+1 else Node r2 x2 t kr.+1
+    merge t1 t2 = match t1 with
+                  | Leaf => t2
+                  | Node l1 x1 r1 _ =>
+                    match t2 with
+                    | Leaf => t1
+                    | Node l2 x2 r2 _ =>
+                      if leT x1 x2
+                      then
+                        if rank (merge r1 t2) <= rank l1
+                        then Node (merge r1 t2) x1 l1 (succn (rank (merge r1 t2)))
+                        else Node l1 x1 (merge r1 t2) (succn (rank l1))
+                      else
+                        if rank (merge t1 r2) <= rank l2
+                        then Node (merge t1 r2) x2 l2 (succn (rank (merge t1 r2)))
+                        else Node l2 x2 (merge t1 r2) (succn (rank l2))
+                    end
                   end.
   Proof. by rewrite /merge pair_merge_equation. Qed.
 
@@ -94,24 +100,11 @@ Module LeftistHeap (Import M: TOTAL_ORDER).
   Fact merge_size t1 t2: size (merge t1 t2) = size t1 + size t2.
   Proof.
     elim: t1 t2 => [|l1 IHl1 x1 r1 IHr1 k1]; elim => [|l2 IHl2 x2 r2 IHr2 k2]; leftist_simpl => //.
-    by case: ifP => ?; case: ifP => ? /=; rewrite ?IHl1 ?IHr1 ?IHl2 ?IHr2 /=; ring.
+    case: ifP => ?; case: ifP => ? /=; rewrite ?IHl1 ?IHr1 ?IHl2 ?IHr2 /=; ring.
   Qed.
 
   Fact insert_size x t: size (insert x t) = (size t).+1.
   Proof. by rewrite merge_size /=; ring. Qed.
-
-  Inductive left_biased: tree -> Prop :=
-  | left_biased_leaf: left_biased Leaf
-  | left_biased_node l x r k: size r <= size l -> left_biased l -> left_biased r -> left_biased (Node l x r k).
-
-  Fact merge_bias t1 t2: left_biased t1 -> left_biased t2 -> left_biased (merge t1 t2).
-  Proof.
-    elim: t1 t2 => [|l1 IHl1 x1 r1 IHr1 k1]; elim => [|l2 IHl2 x2 r2 IHr2 k2]; leftist_simpl => // H1 H2.
-    inversion H1 as [|? ? ? ? ? Hl1 Hr1]; inversion H2 as [|? ? ? ? ? Hl2 Hr2]; subst.
-    move: IHl2 IHr2 => /(_ H1 Hl2) IHl2 /(_ H1 Hr2) IHr2.
-    case: ifP => ?; case: ifP => ?. constructor.
-    - 
-  Admitted.
 
   Fixpoint is_heap t :=
     match t with
@@ -167,13 +160,13 @@ Module LeftistHeap (Import M: TOTAL_ORDER).
       + inversion Hl as [|llb ll lx lr lk Hl0 Hl1 Hl2 Hl3 Hl4]; first by subst.
         subst; case: Hl4 => *; subst.
         have: is_heap (Node t1l t1x t1r t1k) by apply: IHt1; constructor.
-          by simpl; move/andP => [-> ->]; rewrite !andbT.
+        by simpl; move/andP => [-> ->]; rewrite !andbT.
       + inversion Hr as [|rlb rl rx rr rk Hr0 Hr1 Hr2 Hr3 Hr4]; first by subst.
         inversion Hl as [|llb ll lx lr lk Hl0 Hl1 Hl2 Hl3 Hl4]; first by subst.
         subst; case: Hr4; case: Hl4 => *; subst.
         have: is_heap (Node t1l t1x t1r t1k) by apply: IHt1; constructor.
         have: is_heap (Node t2l t2x t2r t2k) by apply: IHt2; constructor.
-          by simpl; do !move/andP => [-> ->]; rewrite !andbT; apply/andP.
+        by simpl; do !move/andP => [-> ->]; rewrite !andbT; apply/andP.
   Qed.
 
   Fact nil_is_heap: is_heap nil.
@@ -192,15 +185,19 @@ Module LeftistHeap (Import M: TOTAL_ORDER).
     | Node l x r _ => Split_min_rest x (merge l r)
     end.
 
-  Function fold {A: Type} (f: T -> A -> A) (a: A) t {measure size t} :=
-    match (split_min t) with
-    | Split_empty => a
-    | Split_min_rest m t' => fold f (f m a) t'
-    end.
-  Proof.
-    move => A f a; case => //= t1 x t2 _ m t'' [? ?]; subst.
-    by apply/ltP; rewrite merge_size.
-  Qed.
+  Section Fold.
+    Variable A: Type.
+    Variable f: T -> A -> A.
+
+    Function fold (a: A) t {measure size t} :=
+      match t with
+      | Leaf => a
+      | Node l x r t' => fold (f x a) (merge l r)
+      end.
+    Proof. by move => *; rewrite merge_size. Qed.
+  End Fold.
+
+  Arguments fold {A}.
 
   Hint Rewrite (fun A f a => fold_equation A f a Leaf)
        (fun A f a l x r k => fold_equation A f a (Node l x r k))
@@ -209,56 +206,79 @@ Module LeftistHeap (Import M: TOTAL_ORDER).
   Definition min x0 t := if t is Node _ x _ _ then x else x0.
   Definition drop_min t := if t is Node l _ r _ then merge l r else Leaf.
 
+  Lemma min_correct t x0: ~ empty t -> heapified t  -> lowerbound (min x0 t) t.
+  Proof.
+    case t => //= l x r k _ H; inversion H; subst.
+    constructor => //; exact: reflexivity.
+  Qed.
+
   Fact min_empty t x0: is_empty t -> min x0 t = x0.
   Proof. by move/emptyP; case. Qed.
 
   Fact min_singleton x x0: min x0 (singleton x) = x.
   Proof. done. Qed.
 
+  Fact lowerboundW {lb lb' t}: leT lb' lb -> lowerbound lb t -> lowerbound lb' t.
+  Proof.
+    case: t => [|l x r k] L; first by constructor.
+    move => H; inversion H; subst; constructor => //.
+    exact: (transitivity lb).
+  Qed.
+
+  Fact lowerbound_merge x t1 t2: lowerbound x t1 -> lowerbound x t2 -> lowerbound x (merge t1 t2).
+  Proof.
+    elim: t1 t2 x => [|t1l IHt1l t1x t1r IHt1r t1k] t2; first by leftist_simpl.
+    elim: t2 => [|t2l IHt2l t2x t2r IHt2r t2k] x; first by leftist_simpl.
+    move => LB1 LB2.
+    inversion LB1; subst; leftist_simpl => //.
+    inversion LB2; subst; leftist_simpl => //.
+    case: ifP => [|/negP] L; case: ifP => R; constructor => //.
+    1,2: by apply: IHt1r => //; constructor => //.
+    all: by apply: IHt2r => //; constructor => //; have [/orP[]]: leT t2x t1x || leT t1x t2x by exact: totality.
+  Qed.
+
+  Hint Resolve lowerbound_merge : leftist.
+
   Fact merge_preserve_heap t1 t2: is_heap t1 -> is_heap t2 -> is_heap (merge t1 t2).
   Proof.
-    move => /heapifiedP H1 /heapifiedP H2; apply/heapifiedP; move: H1 H2.
-    apply: (pair_merge_ind (fun ts t =>forall t1 t2, ts = (t1, t2) -> heapified t1 -> heapified t2 -> heapified t)) => //= {t1 t2}.
-    - by move => [? ?] ? [? ?] ? ? [? ?]; subst.
-    - by move => [? ?]; case => // ? ? ? ? [? ?] _ ? ? [? ?]; subst.
-    - move => [? ?] ? ? r1 ? ? ? ? ? [? ?] ? /(_ r1) IH ? ? ? [? ?] H1 H2; subst.
-      inversion H1; inversion H2; subst.
-      constructor.
-      match goal with
-      | [ |- context[pair_merge (?t1, ?t2)] ] =>
-        suff: heapified (pair_merge (t1, t2))
-      end.
-      move => H; inversion H; constructor.
-      
-      
-    (*   apply: (pair_merge_ind (fun ts t =>forall t1 t2, ts = (t1, t2) -> is_heap t1 -> is_heap t2 -> is_heap t)) => //=. *)
-    (* - by move => [? ?] ? [? ?] ? ? [? ?]; subst. *)
-    (* - move => [? ?] t [? ?]; subst. *)
-    (*     by case t => //= ? ? ? ? _ ? ? [? ?]; subst. *)
-    (* - move => [l r]; case. *)
-    (*   + move => x1 r1 k l2 x2 r2 k2 [? ?] H /(_ r1 r) IH ? ? ? [? ?]; subst => /=  H1' H2'. *)
-    (*     match goal with *)
-    (*     | [ |- context[pair_merge ?ts] ] => case: (pair_merge ts) => // *)
-    (*     end. *)
-    (*     move => ? ? ? ?. *)
+    move => /heapifiedP H1 /heapifiedP H2; apply/heapifiedP.
+    inversion H1 as [|l1 x1 r1 k1 H1l H1r]; subst; first by leftist_simpl.
+    inversion H2 as [|l2 x2 r2 k2 H2l H2r]; subst; first by leftist_simpl.
+    leftist_simpl.
+    case: ifP => [|/negP] L; case: ifP => R; auto with leftist.
+    all: have [/orP[] //]: leT x1 x2  || leT x2 x1 by exact: totality.
+    all: auto with leftist.
+  Qed.
 
-  Admitted.
-
-  Definition to_seq t := rev (fold (seq T) cons [:: ] t).
+  Definition to_seq t := rev (fold cons [:: ] t).
 
   Hint Unfold to_seq : leftist.
 
   Definition from_seq s := seq.foldr insert nil s.
-
 End LeftistHeap.
 
-Module Import NatLeqLeftistHeap := LeftistHeap NatOrder.Leq.
+Module NatOrd <: S.
+  Definition T := nat.
+  Definition leT := leq.
+  Definition leT_total_preorder := ordering.Nat.Leq.
+End NatOrd.
+
+Module Import NatLeftistHeap := LeftistHeap NatOrd.
 
 Example test01: to_seq (merge (singleton 1) (singleton 2)) = [:: 1; 2].
-Proof. by leftist_simpl. Qed.
+Proof. by leftist_simpl; compute. Qed.
 
 Example test02: to_seq (merge (singleton 2) (singleton 1)) = [:: 1; 2].
-Proof. by leftist_simpl. Qed.
+Proof. by leftist_simpl; compute. Qed.
 
-Example test03: to_seq (from_seq [:: 6; 9; 3; 2; 0; 1; 4; 8; 5; 7]) = iota 0 10.
-Proof. by leftist_simpl. Qed.
+
+Function to_seq_naive t {measure size t}: seq nat :=
+  match t with
+  | Leaf => [:: ]
+  | Node l x r _ => [:: x & to_seq_naive (merge l r) ]
+  end.
+Proof. by move => ? ? ? ? ? ?; subst; rewrite merge_size /=. Qed.
+
+Example test03: to_seq_naive (from_seq [:: 6; 9; 3; 2; 0; 1; 4; 8; 5; 7]) = iota 0 10.
+Proof.
+Admitted.
