Makefile
@@ -1,8 +1,4 @@
-all: Makefile.coq
-	$(MAKE) -f Makefile.coq all
-
-%.vo: %.v Makefile.coq
-	$(MAKE) -f Makefile.coq $@
+-include Makefile.coq
 
 Makefile.coq: _CoqProject
 	coq_makefile -f _CoqProject -o $@
